\documentclass{article}

\usepackage{amsmath, amsfonts, amssymb}
\usepackage{amsthm}
\usepackage{hyperref}
\usepackage{tikz-cd}
\usepackage{graphicx}
\usepackage{enumitem}

\graphicspath{{graphics/}}

\author{Matthew Dupraz}
\title{Elliptic Curves over $\mathbb{C}$ and over Finite Fields}

\newtheorem{theorem}{Theorem}[section]
\newtheorem{corollary}{Corollary}[theorem]
\newtheorem{lemma}[theorem]{Lemma}
\newtheorem{proposition}[theorem]{Proposition}

\theoremstyle{definition}
\newtheorem{definition}{Definition}[section]
\newtheorem*{notation}{Notation}

\theoremstyle{remark}
\newtheorem*{remark}{Remark}

\newcommand{\proj}{\mathbb{P}}
\newcommand{\F}{\mathbb{F}}
\newcommand{\C}{\mathbb{C}}
\newcommand{\R}{\mathbb{R}}
\newcommand{\Q}{\mathbb{Q}}
\newcommand{\N}{\mathbb{N}}
\newcommand{\Z}{\mathbb{Z}}
\newcommand{\T}{\mathbb{T}}
\newcommand{\chr}{\operatorname{char}}
\newcommand{\im}{\operatorname{im}}
\newcommand{\rk}{\operatorname{rk}}
\newcommand{\tr}{\operatorname{tr}}
\newcommand{\res}{\operatorname{res}}
\newcommand{\ord}{\operatorname{ord}}
\newcommand{\End}{\operatorname{End}}
\newcommand{\Hom}{\operatorname{Hom}}
\newcommand{\ts}{\textsuperscript}

\begin{document}

\maketitle

\section{Basic Facts}

\subsection{Weierstrass Equation}

Our main interest are \emph{elliptic curves}, which are curves
in $\proj^2$ of genus 1. These are characterized by the
homogeneous equation
\begin{equation}
	\label{weierstrass-eq-1}
	Y^2Z + aXYZ + bYZ^2 = X^3 + cX^2Z + dXZ^2 + eZ^3
\end{equation}
for some $a, b, c, d, e \in \F$.
Setting $U_Z = \{[X, Y, Z] \in \proj^2 \mid Z \neq 0\}$, we can
study the solutions of (\ref{weierstrass-eq-1}) on
$U_Z$ using the change of coordinates $x = X/Z$
and $y = Y/Z$. We obtain the following equation
\begin{equation}
	\label{weierstrass-eq-2}
	y^2 + axy + by = x^3 + cx^2 + dx + e
\end{equation}
We can further simplify this equation with linear
changes of variables. First notice that if $\chr(\F) \neq 2$,
the left hand side can be
written as
\begin{align*}
	y(y + ax + b) &= (y + \frac{1}{2}(ax + b) - \frac{1}{2}(ax + b))
	(y + \frac{1}{2}(ax + b) + \frac{1}{2}(ax + b))\\
	&= (y + \frac{1}{2}(ax + b))^2 - \frac{1}{4}(ax + b)^2
\end{align*}
Hence by replacing $y$ with $y + \frac{1}{2}(ax + b)$ and
collecting the terms in each monomial, we get an equation
of the form
\begin{equation}
	y^2 = x^3 + \alpha x^2 + \beta x + \gamma
\end{equation}
If $\chr(\F) \neq 3$, we can also get rid of the term in 
$x^2$ with a linear change
of variables. replacing $x$ with $x - \frac{1}{3}\alpha$ yields
\begin{align*}
	y^2 &= (x - \frac{1}{3}\alpha)^3 + \alpha(x-\frac{1}{3}\alpha)^2
	+ \beta(x - \frac{1}{3}\alpha) + \gamma\\
	&= x^3 - \alpha x^2 + \frac{1}{3}\alpha^2 x
	- \frac{1}{27}\alpha^3 + \alpha x^2 - \frac{2}{3}\alpha^2 x
	+ \frac{1}{9}\alpha^3 + \beta x - \frac{1}{3}\alpha \beta
	+ \gamma
\end{align*}
Collecting the terms in each monomial, we get an equation of the
form
\begin{equation}
	y^2 = x^3 + Ax + B
\end{equation}
with $A, B \in \F$.
Plugging back the substitutions $x = X/Z$ and $y = Y/Z$, we obtain
the homogeneous equation
\begin{equation}
	Y^2Z = X^3 + AXZ^2 + BZ^3
\end{equation}

\subsection{Singularities}

We suppose $\F$ is algebraically closed.
	
We have that an elliptic curve $V \subset \proj_2(\F)$
is the projective variety
\begin{equation}
	V = V(X^3 + AXZ^2 + BZ^3 - Y^2Z) = V(F)
\end{equation}
We are interested in the case where the curve is smooth.
By the regular preimage theorem, $V$ is smooth if all its points
are non-singular, i.e. if for all $P = [x, y, z] \in V$,
\begin{equation*}
	\nabla F(P) = 
	\begin{bmatrix}
		3x^2 + Az^2\\
		-2yz\\
		2Axz + 3Bz^2 - y^2
	\end{bmatrix}
	\neq 0
\end{equation*}
If $P = [0, 1, 0]$, then 
\begin{equation*}
	\nabla F(P) = 
	\begin{bmatrix}
		0\\
		0\\
		-1
	\end{bmatrix} \neq 0
\end{equation*}
hence the point at infinity is never singular. It follows
that when looking for singularities, we can consider just
the case where $z \neq 0$, since else we have necessarily $x = 0$
and so $P = [0, 1, 0]$. So if there are any singularities of $V$,
they are on $V \cap U_Z$. So $V$ is non-singular precisely when
$V \cap U_Z$ is non-singular. Using the isomorphism
$V \cap U_Z \to W, [X, Y, Z] \mapsto (\frac{X}{Z}, \frac{Y}{Z})$ it
suffices to study singularities on $W = V(x^3 + Ax + B - y^2)
= V(f)$

Let $\Delta = 4A^3 + 27B^2$ be the discriminant of the polynomial
$g(x) = x^3 + Ax + B$, we have the following criteria for the
existence of singularities of $V$.

\begin{proposition}
	W (and equivalently V)
	is non-singular if and only if $\Delta \neq 0$.
\end{proposition}
\begin{proof}
	Suppose there is a point $P = (x_0, y_0) \in W$ that is singular,
	then we have
	\begin{equation*}
		\begin{bmatrix}
			3x_0^2 + A\\
			-2y_0\\
		\end{bmatrix} = 0
	\end{equation*}
	Hence we have that $g'(x_0) = 3x_0^2 + A = 0$ and $y_0 = 0$.
	In particular, since $P \in W$, also 
	$g(x_0) = 0$, and hence since $g(x_0) = g'(x_0) = 0$,
	$x_0$ is a double root of $g$ and so the discriminant
	$\Delta = 4A^3 + 27B^2$ of $g$ is zero.

	Suppose instead that $\Delta = 0$, then $g$ admits a double root
	$x_0 \in \F$ (since we supposed $\F$ algebraically closed)
	which is unique since $g$ is a cubic polynomial.
	Then $P = (x_0, 0) \in V$.
	Furthermore,
	\begin{equation*}
		\nabla f(P) =
		\begin{bmatrix}
			3x^2 + A\\
			0\\
		\end{bmatrix}
	\end{equation*}
	We have that $3x^2 + A = g'(x) = 0$, hence $\nabla f(P) = 0$
	and so $W$ is singular at $P$.
\end{proof}

\include{complex_numbers}
\include{finite_fields}

\end{document}
